ulib/FStar.Monotonic.RRef.fst
@@ -14,45 +14,45 @@ abstract type m_rref (r:rid) (a:Type) (b:reln a) = rref r a
 val as_rref: #r:rid -> #a:Type -> #b:reln a -> m_rref r a b -> GTot (rref r a)
 let as_rref #r #a #b x = x
 
-val contains : #r:rid -> #a:Type -> #b:reln a -> r:m_rref r a b -> m:t -> GTot bool
-let contains #r #a #b r m = HyperHeap.contains_ref (as_rref r) m 
+val m_contains : #r:rid -> #a:Type -> #b:reln a -> r:m_rref r a b -> m:t -> GTot bool
+let m_contains #r #a #b r m = HyperHeap.contains_ref (as_rref r) m 
 
-val sel: #r:rid -> #a:Type -> #b:reln a -> h:t -> m_rref r a b -> GTot a
-let sel #r #a #b h m = HyperHeap.sel h m
+val m_sel: #r:rid -> #a:Type -> #b:reln a -> h:t -> m_rref r a b -> GTot a
+let m_sel #r #a #b h m = HyperHeap.sel h m
 
-val upd: #r:rid -> #a:Type -> #b:reln a -> h:t -> m_rref r a b -> a -> GTot t
-let upd #r #a #b h m v = HyperHeap.upd h m v
+val m_upd: #r:rid -> #a:Type -> #b:reln a -> h:t -> m_rref r a b -> a -> GTot t
+let m_upd #r #a #b h m v = HyperHeap.upd h m v
 
-val ralloc: #a:Type
+val m_alloc: #a:Type
           -> #b:reln a
 	  -> r:rid
           -> init:a
           -> ST (m_rref r a b)
                (requires (fun _ -> monotonic a b))
 	       (ensures (fun h0 (m:m_rref r a b) h1 -> ralloc_post r init h0 (as_rref m) h1))
-let ralloc #a #b r init = ST.ralloc r init
+let m_alloc #a #b r init = ST.ralloc r init
 
-val read:#r:rid 
+val m_read:#r:rid 
        -> #a:Type
        -> #b:reln a
        -> x:m_rref r a b
        -> ST a
             (requires (fun h -> True))
             (ensures (deref_post (as_rref x)))
-let read #r #a #b x = !x
+let m_read #r #a #b x = !x
 
-val write:#r:rid 
+val m_write:#r:rid 
         -> #a:Type
         -> #b:reln a
         -> x:m_rref r a b
         -> v:a
         -> ST unit
-              (requires (fun h0 -> b (sel h0 x) v))
+              (requires (fun h0 -> b (m_sel h0 x) v))
               (ensures (assign_post (as_rref x) v))
-let write #r #a #b x v = x := v
+let m_write #r #a #b x v = x := v
 
 inline type stable_on_t (#i:rid) (#a:Type) (#b:reln a) (r:m_rref i a b) (p:(t -> GTot Type0)) =
-  forall h0 h1. p h0 /\ b (sel h0 r) (sel h1 r) ==> p h1
+  forall h0 h1. p h0 /\ b (m_sel h0 r) (m_sel h1 r) ==> p h1
 abstract type witnessed (p:(t -> GTot Type0)) = True
 
 val witness: #r:rid
@@ -65,8 +65,15 @@ val witness: #r:rid
                 (ensures (fun h0 _ h1 -> h0=h1 /\ witnessed p))
 let witness #r #a #b m p = ()
 
-val recall: p:(t -> GTot Type0)
+val testify: p:(t -> GTot Type0)
           -> ST unit
                (requires (fun _ ->  witnessed p))
                (ensures (fun h0 _ h1 -> p h1))
-let recall p = admit() //intentionally admitted
+let testify p = admit() //intentionally admitted
+
+val m_recall: #r:rid -> #a:Type -> #b:reln a 
+            -> m:m_rref r a b
+	    -> ST unit 
+	      (requires (fun h -> True))
+	      (ensures (fun h0 _ h1 -> h0=h1 /\ m_contains m h1))
+let m_recall #r #a #b m = admit() //intentionally admitted
